migrating SQRL

Examples/SQRL_Shorewall/Analyze_SQRL_Shorewall.thy
@@ -14,7 +14,6 @@ local_setup \<open>
  \<close>
 
 thm SQRL_fw_def
-
 thm SQRL_fw_FORWARD_default_policy_def
 
 value[code] "map (\<lambda>(c,rs). (c, map (quote_rewrite \<circ> common_primitive_rule_toString) rs)) SQRL_fw"
@@ -25,15 +24,26 @@ lemma "Semantics_Goto.terminal_chain (the ((map_of_string SQRL_fw) ''reject''))"
 
 value[code] "Semantics_Goto.rewrite_Goto SQRL_fw"
 
+definition "unfolded = unfold_ruleset_FORWARD SQRL_fw_FORWARD_default_policy (map_of_string (Semantics_Goto.rewrite_Goto SQRL_fw))"
+
+(*31.053s*)
+value[code] "unfolded"
+(*2.871s*)
+lemma "length unfolded = 2649" by eval
+
 (*11.918s*)
-value[code] "map (quote_rewrite \<circ> common_primitive_rule_toString) 
-               (upper_closure (unfold_ruleset_FORWARD SQRL_fw_FORWARD_default_policy (map_of_string (Semantics_Goto.rewrite_Goto SQRL_fw))))" 
+value[code] "map (quote_rewrite \<circ> common_primitive_rule_toString) (upper_closure unfolded)"
+lemma "length (upper_closure unfolded) = 1683" by eval
+
+(*53.507s*)
+lemma "length (lower_closure unfolded) = 14138" by eval
 
 
 (*16.334s*)
-value[code] "map simple_rule_toString
-              (to_simple_firewall
-               (upper_closure (unfold_ruleset_FORWARD SQRL_fw_FORWARD_default_policy (map_of_string (Semantics_Goto.rewrite_Goto SQRL_fw)))))" 
+value[code] "map simple_rule_toString (to_simple_firewall (upper_closure unfolded))" 
+lemma "length (to_simple_firewall (upper_closure unfolded)) = 1683" by eval
+(*81.437s*)
+lemma "length (to_simple_firewall (lower_closure unfolded)) = 11212" by eval
 
 
 export_code unfold_ruleset_FORWARD map_of_string upper_closure lower_closure
